src/Ren.v
@@ -181,3 +181,5 @@ Qed.
 Definition wk {Γ τ τ'} : Exp Γ τ → Exp (τ' :: Γ) τ := RenExp skip1.
 
 End Ren.
+
+Extraction RcR.
